Test/Prop/Assoc.lean
@@ -2,5 +2,5 @@ import Smt
 
 theorem assoc (f : Prop → Prop → Prop) (p q r : Prop) :
   f p (f q r) = f (f p q) r := by
-  smt
+  smt +model
   admit
