Test/Prop/Comm.lean
@@ -1,5 +1,5 @@
 import Smt
 
 example (f : Prop → Prop → Prop) (p q : Prop) : f p q = f q p := by
-  smt
+  smt +model
   admit
